update hash definition

tests/sha2-mb-test.c
@@ -41,11 +41,11 @@ print_test1(uint8_t* in, int in_len, uint8_t* exp256, uint8_t* exp512)
   uint8_t comp256[32] = { 0 };
   uint8_t comp512[64] = { 0 };
 
-  Hacl_Streaming_SHA2_sha256(in, in_len, comp256);
+  Hacl_Streaming_SHA2_sha256(comp256, in, in_len);
   printf("NEW SHA2-256 (32-bit) Result:\n");
   bool ok = print_result(comp256, exp256, 32);
 
-  Hacl_Streaming_SHA2_sha512(in, in_len, comp512);
+  Hacl_Streaming_SHA2_sha512(comp512, in, in_len);
   printf("NEW SHA2-512 (32-bit) Result:\n");
   ok = print_result(comp512, exp512, 64) && ok;
 
@@ -232,13 +232,13 @@ main()
   memset(plain, 'P', SIZE);
 
   for (int j = 0; j < ROUNDS; j++) {
-    Hacl_Streaming_SHA2_sha256(plain, SIZE, plain);
+    Hacl_Streaming_SHA2_sha256(plain, plain, SIZE);
   }
 
   t1 = clock();
   a = cpucycles_begin();
   for (int j = 0; j < ROUNDS; j++) {
-    Hacl_Streaming_SHA2_sha256(plain, SIZE, plain);
+    Hacl_Streaming_SHA2_sha256(plain, plain, SIZE);
   }
   b = cpucycles_end();
   t2 = clock();
@@ -328,13 +328,13 @@ main()
 #endif
 
   for (int j = 0; j < ROUNDS; j++) {
-    Hacl_Streaming_SHA2_sha512(plain, SIZE, plain);
+    Hacl_Streaming_SHA2_sha512(plain, plain, SIZE);
   }
 
   t1 = clock();
   a = cpucycles_begin();
   for (int j = 0; j < ROUNDS; j++) {
-    Hacl_Streaming_SHA2_sha512(plain, SIZE, plain);
+    Hacl_Streaming_SHA2_sha512(plain, plain, SIZE);
   }
   b = cpucycles_end();
   t2 = clock();
